Fsub_Lemmas.v
@@ -21,8 +21,10 @@
       - #<a href="##regularity">Regularity lemmas</a>#
       - #<a href="##auto">Automation</a># *)
 
-Require Export Fsub_Infrastructure.
+Require Import Coq.Program.Equality.
 
+Require Export Fsub_Infrastructure.
+Require Import Atom.
 
 (* ********************************************************************** *)
 (** * #<a name="wft"></a># Properties of [wf_typ] *)
@@ -30,23 +32,26 @@ Require Export Fsub_Infrastructure.
 (** If a type is well-formed in an environment, then it is locally
     closed. *)
 
-Lemma capt_from_wf_cset : forall E C,
-  wf_cset E C -> capt C.
+Lemma capt_from_wf_cset : forall E A C,
+  wf_cset E A C -> capt C.
 Proof with auto.
   intros.
   inversion H...
 Qed.
 
-Lemma type_from_wf_typ : forall E T,  
-  wf_typ E T -> type T
-with pretype_from_wf_pretyp : forall E T,
-  wf_pretyp E T -> pretype T.
+Lemma type_from_wf_typ : forall E Ap Am T,
+  wf_typ E Ap Am T -> type T
+with pretype_from_wf_pretyp : forall E Ap Am T,
+  wf_pretyp E Ap Am T -> pretype T.
 Proof with eauto using capt_from_wf_cset.
 ------
-  intros E T H; induction H.
-  econstructor. econstructor...
+  intros *. intros H.
+  induction H.
+  econstructor.
+  econstructor...
 ------
-  intros E T H; induction H.
+  intros *. intros H.
+  induction H.
   - trivial.
   - pick fresh X and apply type_arrow...
   - pick fresh X and apply type_all...
@@ -56,10 +61,10 @@ Qed.
     capture set wellformedness. *)
 
 Ltac wf_cset_simpl instantiate_ext :=
-  match goal with 
-  | H : _ |- (wf_cset _ cset_universal) =>
+  match goal with
+  | H : _ |- (wf_cset _ _ cset_universal) =>
     constructor
-  | H : (wf_cset _ ?C) |- (wf_cset _ ?C) =>
+  | H : (wf_cset _ _ ?C) |- (wf_cset _ _ ?C) =>
     let Hdestruct := fresh "Hdestruct" in
     let x  := fresh "x" in
     let Hx := fresh "Hxin" in
@@ -67,52 +72,64 @@ Ltac wf_cset_simpl instantiate_ext :=
     let T := fresh "T" in
     let Hbound := fresh "Hbound" in
     let E := fresh "E" in
+    let A := fresh "A" in
     let fvars := fresh "fvars" in
     let Hclosed := fresh "Hclosed" in
-      inversion H as [|E fvars Hbound Hclosed]; subst; [ auto | 
-        constructor;
+    inversion H as [|E A fvars Hbound Hclosed]; subst; [
+      auto |
+      constructor; [
         unfold allbound_typ in Hbound;
         intros x Hx;
         destruct (Hbound x Hx) as [T Hexists];
         lazymatch instantiate_ext with
         | True => exists T
         | False => idtac
-      end ]
+        end |
+        fsetdec
+      ]
+    ]
   end.
-  
-Lemma wf_cset_weakening : forall E F G C,
-    wf_cset (G ++ E) C ->
+
+Lemma wf_cset_weakening : forall E A A' F G C,
+    wf_cset (G ++ E) A C ->
     ok (G ++ F ++ E) ->
-    wf_cset (G ++ F ++ E) C.
+    AtomSet.F.Subset A A' ->
+    wf_cset (G ++ F ++ E) A' C.
 Proof with auto*.
-  intros E F G C Hcset Henv.
+  intros *.
+  intros Hcset Henv Hpres.
   wf_cset_simpl True...
 Qed.
 
-Lemma wf_cset_weaken_head : forall C E F,
-  wf_cset E C ->
+Lemma wf_cset_weaken_head : forall C E A F,
+  wf_cset E A C ->
   ok (F ++ E) ->
-  wf_cset (F ++ E) C.
+  wf_cset (F ++ E) A C.
 Proof.
   intros.
   rewrite_env (empty ++ F++ E).
-  auto using wf_cset_weakening.
+  apply wf_cset_weakening with (A := A); auto.
+  fsetdec.
 Qed.
 
-Lemma wf_typ_weakening : forall T E F G,
-  wf_typ (G ++ E) T ->
+Lemma wf_typ_weakening : forall T E Ap Am Ap' Am' F G,
+  wf_typ (G ++ E) Ap Am T ->
   ok (G ++ F ++ E) ->
-  wf_typ (G ++ F ++ E) T
-with wf_pretyp_weakening : forall T E F G,
-  wf_pretyp (G ++ E) T ->
+  AtomSet.F.Subset Ap Ap' ->
+  AtomSet.F.Subset Am Am' ->
+  wf_typ (G ++ F ++ E) Ap' Am' T
+with wf_pretyp_weakening : forall T E Ap Am Ap' Am' F G,
+  wf_pretyp (G ++ E) Ap Am T ->
   ok (G ++ F ++ E) ->
-  wf_pretyp (G ++ F ++ E) T.
+  AtomSet.F.Subset Ap Ap' ->
+  AtomSet.F.Subset Am Am' ->
+  wf_pretyp (G ++ F ++ E) Ap' Am' T.
 Proof with simpl_env; eauto using wf_cset_weakening.
 ------
   intros.
   remember (G ++ E).
   generalize dependent G.
-  induction H; intros G Hok Heq; subst. 
+  induction H; intros G Hok Heq; subst.
   - apply wf_typ_var with (U := U)...
   - apply wf_typ_capt...
 ------
@@ -123,46 +140,66 @@ Proof with simpl_env; eauto using wf_cset_weakening.
   - apply wf_typ_top.
   (* typ_arrow case *)
   - pick fresh Y and apply wf_typ_arrow.
-    apply wf_typ_weakening...
+    eapply wf_typ_weakening...
     rewrite <- concat_assoc.
-    apply wf_typ_weakening...
+    eapply wf_typ_weakening...
+    Set Nested Proofs Allowed.
+    Local Lemma just_do_it : forall A B C,
+        AtomSet.F.Subset A B ->
+        AtomSet.F.Subset (A `union` C) (B `union` C).
+    Proof.
+      intros.
+      fsetdec.
+    Qed.
+    apply just_do_it.
+    fsetdec.
   (* typ_all case *)
   - pick fresh Y and apply wf_typ_all.
-    apply wf_typ_weakening...
+    eapply wf_typ_weakening...
     rewrite <- concat_assoc.
-    apply wf_typ_weakening...
+    eapply wf_typ_weakening...
 Qed.
 
-Lemma wf_typ_weaken_head : forall T E F,
-  wf_typ E T ->
+Lemma wf_typ_weaken_head : forall T E Ap Am Ap' Am' F,
+  wf_typ E Ap Am T ->
   ok (F ++ E) ->
-  wf_typ (F ++ E) T.
+  AtomSet.F.Subset Ap Ap' ->
+  AtomSet.F.Subset Am Am' ->
+  wf_typ (F ++ E) Ap' Am' T.
 Proof.
   intros.
   rewrite_env (empty ++ F ++ E).
-  auto using wf_typ_weakening.
+  apply wf_typ_weakening with (Ap := Ap) (Am := Am); eauto || fsetdec.
 Qed.
 
-
 (* Type bindings don't matter at all! *)
-Lemma wf_cset_narrowing : forall V U C E F X,
-  wf_cset (F ++ [(X, bind_sub V)] ++ E) C ->
+Lemma wf_cset_narrowing : forall V U C E A F X,
+  wf_cset (F ++ [(X, bind_sub V)] ++ E) A C ->
   ok (F ++ [(X, bind_sub U)] ++ E) ->
-  wf_cset (F ++ [(X, bind_sub U)] ++ E) C.
+  wf_cset (F ++ [(X, bind_sub U)] ++ E) A C.
 Proof with simpl_env; eauto.
-  intros V U C E F X Hwf Hok.
+  intros *.
+  intros Hwf Hok.
   wf_cset_simpl True...
   binds_cases Hexists...
 Qed.
 
-Lemma wf_typ_narrowing : forall V U T E F X,
-  wf_typ (F ++ [(X, bind_sub V)] ++ E) T ->
+Lemma wf_typ_narrowing : forall V U T E Ap Am F X,
+  wf_typ (F ++ [(X, bind_sub V)] ++ E) Ap Am T ->
   ok (F ++ [(X, bind_sub U)] ++ E) ->
-  wf_typ (F ++ [(X, bind_sub U)] ++ E) T
-with wf_pretyp_narrowing : forall V U T E F X,
-  wf_pretyp (F ++ [(X, bind_sub V)] ++ E) T ->
+  wf_typ (F ++ [(X, bind_sub U)] ++ E) Ap Am T
+with wf_pretyp_narrowing : forall V U T E Ap Am F X,
+  wf_pretyp (F ++ [(X, bind_sub V)] ++ E) Ap Am T ->
   ok (F ++ [(X, bind_sub U)] ++ E) ->
-  wf_pretyp (F ++ [(X, bind_sub U)] ++ E) T.
+  wf_pretyp (F ++ [(X, bind_sub U)] ++ E) Ap Am T.
+(* Lemma wf_typ_narrowing : forall V U T E F X, *)
+(*   wf_typ_in (F ++ [(X, bind_sub V)] ++ E) T -> *)
+(*   ok (F ++ [(X, bind_sub U)] ++ E) -> *)
+(*   wf_typ_in (F ++ [(X, bind_sub U)] ++ E) T *)
+(* with wf_pretyp_narrowing : forall V U T E F X, *)
+(*   wf_pretyp_in (F ++ [(X, bind_sub V)] ++ E) T -> *)
+(*   ok (F ++ [(X, bind_sub U)] ++ E) -> *)
+(*   wf_pretyp_in (F ++ [(X, bind_sub U)] ++ E) T. *)
 Proof with simpl_env; eauto using wf_cset_narrowing.
 ------
   intros.
@@ -182,7 +219,7 @@ Proof with simpl_env; eauto using wf_cset_narrowing.
   induction H; intros F Hok Heq; subst; try solve [econstructor].
   (* typ_arrow *)
   - pick fresh Y and apply wf_typ_arrow...
-   rewrite <- concat_assoc.
+    rewrite <- concat_assoc.
     eapply wf_typ_narrowing...
   (* typ_all *)
   - pick fresh Y and apply wf_typ_all...
@@ -190,36 +227,35 @@ Proof with simpl_env; eauto using wf_cset_narrowing.
     eapply wf_typ_narrowing...
 Qed.
 
-
 (* JONATHAN: Maybe those _sub variants are not needed afterall! *)
-Lemma wf_cset_narrowing_typ : forall C1 C2 C E F X,
-  wf_cset (F ++ [(X, bind_typ C1)] ++ E) C ->
+Lemma wf_cset_narrowing_typ : forall C1 C2 C E A F X,
+  wf_cset (F ++ [(X, bind_typ C1)] ++ E) A C ->
   ok (F ++ [(X, bind_typ C2)] ++ E) ->
-  wf_cset (F ++ [(X, bind_typ C2)] ++ E) C.
+  wf_cset (F ++ [(X, bind_typ C2)] ++ E) A C.
 Proof with simpl_env; eauto.
-  intros C1 C2 C E F X Hwf Hok.
+  intros *. intros Hwf Hok.
   wf_cset_simpl False.
   binds_cases Hexists...
 Qed.
 
-Lemma wf_typ_narrowing_typ : forall C1 C2 T E F X,
-  wf_typ (F ++ [(X, bind_typ C1)] ++ E) T ->
+Lemma wf_typ_narrowing_typ : forall C1 C2 T E Ap Am F X,
+  wf_typ (F ++ [(X, bind_typ C1)] ++ E) Ap Am T ->
   ok (F ++ [(X, bind_typ C2)] ++ E) ->
-  wf_typ (F ++ [(X, bind_typ C2)] ++ E) T
-with wf_pretyp_narrowing_typ : forall C1 C2 T E F X,
-  wf_pretyp (F ++ [(X, bind_typ C1)] ++ E) T ->
+  wf_typ (F ++ [(X, bind_typ C2)] ++ E) Ap Am T
+with wf_pretyp_narrowing_typ : forall C1 C2 T E Ap Am F X,
+  wf_pretyp (F ++ [(X, bind_typ C1)] ++ E) Ap Am T ->
   ok (F ++ [(X, bind_typ C2)] ++ E) ->
-  wf_pretyp (F ++ [(X, bind_typ C2)] ++ E) T.
+  wf_pretyp (F ++ [(X, bind_typ C2)] ++ E) Ap Am T.
 Proof with simpl_env; eauto using wf_cset_narrowing_typ.
 ------
-  intros C1 C2 T E F X Hwf_typ Hok.
+  intros *. intros Hwf_typ Hok.
   remember (F ++ [(X, bind_typ C1)] ++ E).
   generalize dependent F.
   induction Hwf_typ; intros F Hok Heq; subst.
   - binds_cases H...
   - econstructor...
 ------
-  intros C1 C2 T E F X Hwf_typ Hok.
+  intros *. intros Hwf_typ Hok.
   remember (F ++ [(X, bind_typ C1)] ++ E).
   generalize dependent F.
   induction Hwf_typ; intros F Hok Heq; subst.
@@ -235,44 +271,68 @@ Proof with simpl_env; eauto using wf_cset_narrowing_typ.
 Qed.
 
 (** Substitution lemmas *)
-Lemma wf_cset_subst_tb : forall F Q E Z P C,
-  wf_cset (F ++ [(Z, bind_sub Q)] ++ E) C ->
-  wf_typ E P ->
+Lemma wf_cset_subst_tb : forall F Q E Ap Am Z P C,
+  wf_cset (F ++ [(Z, bind_sub Q)] ++ E) Ap C ->
+  wf_typ E Ap Am P ->
   ok (map (subst_tb Z P) F ++ E) ->
-  wf_cset (map (subst_tb Z P) F ++ E) C.
+  wf_cset (map (subst_tb Z P) F ++ E) Ap C.
 Proof with simpl_env; eauto*.
-  intros F Q E Z P C HwfC HwfP Hok.
+  intros *. intros HwfC HwfP Hok.
   wf_cset_simpl False...
   binds_cases Hexists...
   * exists (subst_tt Z P T)...
 Qed.
 
-Lemma wf_typ_subst_tb : forall F Q E Z P T,
-  wf_typ (F ++ [(Z, bind_sub Q)] ++ E) T ->
-  (** NOTE here that P needs to be well formed in both the + and - environments,
-      as we're substituting in both places. *)
-  wf_typ E P ->
+Lemma come_on : forall E Ap Am Ap' Am' T,
+  wf_typ E Ap Am T ->
+  ok E ->
+  AtomSet.F.Subset Ap Ap' ->
+  AtomSet.F.Subset Am Am' ->
+  wf_typ E Ap' Am' T.
+Proof.
+  intros.
+  rewrite_env (empty ++ empty ++ E).
+  rewrite_env (empty ++ E) in H.
+  eapply wf_typ_weakening; eauto.
+Qed.
+
+Lemma wf_typ_subst_tb : forall F Q E Ap Am Z P T,
+  wf_typ (F ++ [(Z, bind_sub Q)] ++ E) Ap Am T ->
+  (** NOTE here that P needs to be well formed in both the + and - environments, *)
+(*       as we're substituting in both places. *)
+  wf_typ E Ap Am P ->
+  wf_typ E Am Ap P ->
   ok (map (subst_tb Z P) F ++ E) ->
-  wf_typ (map (subst_tb Z P) F ++ E) (subst_tt Z P T)
-with wf_pretyp_subst_tb : forall F Q E Z P T,
-  wf_pretyp (F ++ [(Z, bind_sub Q)] ++ E) T ->
-  wf_typ E P ->
+  wf_typ (map (subst_tb Z P) F ++ E) Ap Am (subst_tt Z P T)
+with wf_pretyp_subst_tb : forall F Q E Ap Am Z P T,
+  wf_pretyp (F ++ [(Z, bind_sub Q)] ++ E) Ap Am T ->
+  wf_typ E Ap Am P ->
+  wf_typ E Am Ap P ->
   ok (map (subst_tb Z P) F ++ E) ->
-  wf_pretyp (map (subst_tb Z P) F ++ E) (subst_tpt Z P T).
+  wf_pretyp (map (subst_tb Z P) F ++ E) Ap Am (subst_tpt Z P T).
 Proof with simpl_env; eauto using wf_typ_weaken_head, type_from_wf_typ, wf_cset_subst_tb.
 ------
-  intros F Q E Z P T HwfT HwfP Hok.
+  intros *. intros HwfT HwfPp HwfPm Hok.
   remember (F ++ [(Z, bind_sub Q)] ++ E).
   generalize dependent F.
   induction HwfT; intros F EQF Hok; subst; simpl subst_tt.
   - Case "wf_typ_var".
     destruct (X == Z); subst...
+    + rewrite_env (empty ++ map (subst_tb Z P) F ++ E).
+      eapply wf_typ_weakening.
+      1: {
+        simpl_env.
+        apply HwfPp.
+      }
+      all : auto || fsetdec.
     + SCase "X <> Z".
+      unfold wf_typ_in in *.
       binds_cases H...
       apply (wf_typ_var (subst_tt Z P U))...
-  - econstructor...
+  - unfold wf_typ_in in *.
+    econstructor...
 ------
-  intros F Q E Z P T HwfT HwfP Hok.
+  intros *. intros HwfT HwfPp HwfPm Hok.
   remember (F ++ [(Z, bind_sub Q)] ++ E).
   generalize dependent F.
   induction HwfT; intros F EQF Hok; subst; simpl subst_tt.
@@ -284,6 +344,18 @@ Proof with simpl_env; eauto using wf_typ_weaken_head, type_from_wf_typ, wf_cset_
       rewrite <- subst_tt_open_ct_rec...
       rewrite_env (map (subst_tb Z P) ([(Y, bind_typ T1)] ++ F) ++ E).
       eapply wf_typ_subst_tb...
+      * apply come_on with (Ap := Ap) (Am := Am)...
+        ** rewrite_env (empty ++ E).
+           rewrite_env (empty ++ map (subst_tb Z P) F ++ E) in Hok.
+           eapply ok_remove_mid...
+        ** fsetdec.
+        ** fsetdec.
+      * apply come_on with (Ap := Am) (Am := Ap)...
+        ** rewrite_env (empty ++ E).
+           rewrite_env (empty ++ map (subst_tb Z P) F ++ E) in Hok.
+           eapply ok_remove_mid...
+        ** fsetdec.
+        ** fsetdec.
   - Case "wf_typ_all".
     pick fresh Y and apply wf_typ_all...
     + SCase "T2".
@@ -291,21 +363,33 @@ Proof with simpl_env; eauto using wf_typ_weaken_head, type_from_wf_typ, wf_cset_
       rewrite subst_tt_open_tt_var...
       rewrite_env (map (subst_tb Z P) ([(Y, bind_sub T1)] ++ F) ++ E).
       eapply wf_typ_subst_tb...
+      (* * apply come_on with (Ap := Ap) (Am := Am)... *)
+      (*   ** rewrite_env (empty ++ E). *)
+      (*      rewrite_env (empty ++ map (subst_tb Z P) F ++ E) in Hok. *)
+      (*      eapply ok_remove_mid... *)
+      (*   ** fsetdec. *)
+      (*   ** fsetdec. *)
+      (* * apply come_on with (Ap := Am) (Am := Ap)... *)
+      (*   ** rewrite_env (empty ++ E). *)
+      (*      rewrite_env (empty ++ map (subst_tb Z P) F ++ E) in Hok. *)
+      (*      eapply ok_remove_mid... *)
+      (*   ** fsetdec. *)
+      (*   ** fsetdec. *)
 Qed.
 
-Lemma wf_typ_open : forall E U T1 T2,
-  ok E ->
-  wf_pretyp E (typ_all T1 T2) ->
-  wf_typ E U ->
-  wf_typ E (open_tt T2 U).
-Proof with simpl_env; eauto.
-  intros E U T1 T2 O WA WU.
-  inversion WA; subst.
-  pick fresh X.
-  rewrite (subst_tt_intro X)...
-  rewrite_env (map (subst_tb X U) empty ++ E).
-  apply wf_typ_subst_tb with (Q := T1)...
-Qed.
+(* Lemma wf_typ_open : forall E U T1 T2, *)
+(*   ok E -> *)
+(*   wf_pretyp E (typ_all T1 T2) -> *)
+(*   wf_typ E U -> *)
+(*   wf_typ E (open_tt T2 U). *)
+(* Proof with simpl_env; eauto. *)
+(*   intros E U T1 T2 O WA WU. *)
+(*   inversion WA; subst. *)
+(*   pick fresh X. *)
+(*   rewrite (subst_tt_intro X)... *)
+(*   rewrite_env (map (subst_tb X U) empty ++ E). *)
+(*   apply wf_typ_subst_tb with (Q := T1)... *)
+(* Qed. *)
 
 (** This should move into infrastructure probably at some point. **)
 (** The next lemma states that opening a term is equivalent to first
@@ -324,7 +408,7 @@ Proof with auto*.
   induction T2; intros C k Fr; simpl in *; f_equal...
   - Case "typ_cset".
     apply subst_capt_cset_swap.
-    csetdec; destruct c...  
+    csetdec; destruct c...
 ------
   induction T2; intros C k Fr; simpl in *; f_equal...
 Qed.
@@ -348,14 +432,14 @@ Lemma subst_open_cset : forall k X C1 C2 c,
 Proof.
   intros.
   unfold subst_cset; unfold open_cset;
-  cset_split; cset_cleanup; 
+  cset_split; cset_cleanup;
   destruct C2 eqn:HC2; destruct C1 eqn:HC1; try destruct c eqn:Hc;
   f_equal; subst; try fsetdec; try fnsetdec.
   all: inversion H; inversion H0; subst; fnsetdec.
 Qed.
 
 (* unfold subst_cset; unfold open_cset;
-  cset_split; cset_cleanup; 
+  cset_split; cset_cleanup;
   destruct C2 eqn:HC2; destruct C1 eqn:HC1; try destruct c eqn:Hc;
   f_equal; subst; try fsetdec; try fnsetdec. *)
 (* all: inversion H; inversion H0; subst; fnsetdec. *)
@@ -374,7 +458,7 @@ Proof with auto using subst_open_cset.
 ------
   intros X C1 T C2.
   induction T; intros; simpl; try trivial.
-  
+
   f_equal.
   - apply subst_open_cset...
   - apply subst_cpt_open_cpt_rec...
@@ -395,129 +479,129 @@ Proof with auto*.
   rewrite subst_ct_open_tt_rec...
 Qed.
 
-Lemma wf_cset_over_subst : forall F Q E Z C C',
-  ok (map (subst_cb Z C) F ++ E) ->
-  wf_cset E C ->
-  wf_cset (F ++ [(Z, bind_typ Q)] ++ E) C' ->
-  ok (F ++ [(Z, bind_typ Q)] ++ E) ->
-  wf_cset (map (subst_cb Z C) F ++ E) (subst_cset Z C C').
-Proof with eauto*.
-  intros F Q E Z C C'.
-  intros HOK HwfC HwfC' HokZ .
-  inversion HwfC; subst; inversion HwfC'; subst...
-  + unfold subst_cset...
-    cset_split...
-    constructor...
-    unfold allbound_typ in * ...
-    intros.
-    specialize (H x H0).
-    rewrite cset_not_references_fvar_eq in H_destruct...
-    csethyp.
-    assert (x <> Z) by fsetdec.
-    inversion H.
-    binds_cases H2...
-    exists (subst_ct Z cset_universal x0)...
-  + unfold subst_cset...
-    cset_split; inversion HwfC; inversion HwfC'; subst; try rewrite cset_not_references_fvar_eq in H_destruct;
-      try rewrite cset_references_fvar_eq in H_destruct;
-      assert (NatSet.F.union {}N {}N = {}N) by (fnsetdec; eauto*);
-      try rewrite H1; constructor; unfold allbound_typ in *; intros...
-    * assert (x `in` (fvars `union` fvars0)) by fsetdec.
-      rewrite AtomSetFacts.union_iff in H4... inversion H4...
-      **
-        specialize (H3 x H5).
-        inversion H3 as [T H7].
-        exists T.
-        apply binds_weaken with (G := nil)...         
-      **
-        specialize (H6 x H5).
-        inversion H6 as [T H7].
-        binds_cases H7; subst...
-        - contradict H2.
-          assert (x `notin` fvars). {
-            intro. specialize (H x H2)...
-            inversion H as [T' H7]...
-            (** Clearly true as x \in fvars0, x \notin fvars \cup (x - fvars0)*)
-            apply fresh_mid_tail in HokZ...
-            apply binds_In in H7...
-          }
-          fsetdec.
-        - exists (subst_ct Z (cset_set fvars {}N) T).
-          eauto*.
-    * 
-      specialize (H6 x H2).
-      inversion H6 as [T H7].
-      binds_cases H7; subst...
-      - exists (subst_ct Z (cset_set fvars {}N) T).
-        eauto*.   
-Qed.
+(* Lemma wf_cset_over_subst : forall F Q E A Z C C', *)
+(*   ok (map (subst_cb Z C) F ++ E) -> *)
+(*   wf_cset E A C -> *)
+(*   wf_cset (F ++ [(Z, bind_typ Q)] ++ E) A C' -> *)
+(*   ok (F ++ [(Z, bind_typ Q)] ++ E) -> *)
+(*   wf_cset (map (subst_cb Z C) F ++ E) A (subst_cset Z C C'). *)
+(* Proof with eauto*. *)
+(*   intros *. *)
+(*   intros HOK HwfC HwfC' HokZ . *)
+(*   inversion HwfC; subst; inversion HwfC'; subst... *)
+(*   + unfold subst_cset... *)
+(*     cset_split... *)
+(*     constructor... *)
+(*     unfold allbound_typ in * ... *)
+(*     intros. *)
+(*     specialize (H x H1). *)
+(*     rewrite cset_not_references_fvar_eq in H_destruct... *)
+(*     csethyp. *)
+(*     assert (x <> Z) by fsetdec. *)
+(*     inversion H. *)
+(*     binds_cases H2... *)
+(*     exists (subst_ct Z cset_universal x0)... *)
+(*   + unfold subst_cset... *)
+(*     cset_split; inversion HwfC; inversion HwfC'; subst; try rewrite cset_not_references_fvar_eq in H_destruct; *)
+(*       try rewrite cset_references_fvar_eq in H_destruct; *)
+(*       assert (NatSet.F.union {}N {}N = {}N) by (fnsetdec; eauto* ); *)
+(*       try rewrite H1; constructor; unfold allbound_typ in *; intros... *)
+(*     * assert (x `in` (fvars `union` fvars0)) by fsetdec. *)
+(*       rewrite AtomSetFacts.union_iff in H4... inversion H4... *)
+(*       ** *)
+(*         specialize (H3 x H5). *)
+(*         inversion H3 as [T H7]. *)
+(*         exists T. *)
+(*         apply binds_weaken with (G := nil)... *)
+(*       ** *)
+(*         specialize (H6 x H5). *)
+(*         inversion H6 as [T H7]. *)
+(*         binds_cases H7; subst... *)
+(*         - contradict H2. *)
+(*           assert (x `notin` fvars). { *)
+(*             intro. specialize (H x H2)... *)
+(*             inversion H as [T' H7]... *)
+(*             (** Clearly true as x \in fvars0, x \notin fvars \cup (x - fvars0)*) *)
+(*             apply fresh_mid_tail in HokZ... *)
+(*             apply binds_In in H7... *)
+(*           } *)
+(*           fsetdec. *)
+(*         - exists (subst_ct Z (cset_set fvars {}N) T). *)
+(*           eauto*. *)
+(*     * *)
+(*       specialize (H6 x H2). *)
+(*       inversion H6 as [T H7]. *)
+(*       binds_cases H7; subst... *)
+(*       - exists (subst_ct Z (cset_set fvars {}N) T). *)
+(*         eauto*. *)
+(* Qed. *)
 
-Lemma wf_typ_subst_cb : forall F Q E Z C T,
-  wf_typ (F ++ [(Z, bind_typ Q)] ++ E) T ->
-  (** NOTE here that P needs to be well formed in both the + and - environments,
-      as we're substituting in both places. *)
-  wf_cset E C ->
-  ok (map (subst_cb Z C) F ++ E) ->
-  ok (F ++ [(Z, bind_typ Q)] ++ E) ->
-  wf_typ (map (subst_cb Z C) F ++ E) (subst_ct Z C T)
-with wf_pretyp_subst_cb : forall F Q E Z C T,
-  wf_pretyp (F ++ [(Z, bind_typ Q)] ++ E) T ->
-  wf_cset E C ->
-  ok (map (subst_cb Z C) F ++ E) ->
-  ok (F ++ [(Z, bind_typ Q)] ++ E) ->
-  wf_pretyp (map (subst_cb Z C) F ++ E) (subst_cpt Z C T).
-Proof with simpl_env; eauto using wf_typ_weaken_head, type_from_wf_typ, wf_cset_subst_tb,
-    capt_from_wf_cset.
-------
-  intros F Q E Z C T HwfT HwfC Hok HokZ.
-  remember (F ++ [(Z, bind_typ Q)] ++ E).
-  generalize dependent F.
-  induction HwfT; intros F EQF Hok; subst; simpl subst_ct...
-  - Case "wf_typ_var".
-      binds_cases H...
-      apply (wf_typ_var (subst_ct Z C U))...  
-  - Case "wf_typ_capt".
-    constructor...
-    apply wf_cset_over_subst with (Q := Q)...
-------
-  intros F Q E Z C T HwfT HwfC Hok HokZ.
-  remember (F ++ [(Z, bind_typ Q)] ++ E).
-  generalize dependent F.
-  induction HwfT; intros F EQF Hok; subst; simpl subst_ct.
-  - constructor.
-  - Case "wf_typ_arrow".
-    pick fresh Y and apply wf_typ_arrow...
-    + SCase "T2".
-      unfold open_ct in *...
-      rewrite <- subst_ct_open_ct_rec...
-      rewrite_env (map (subst_cb Z C) ([(Y, bind_typ T1)] ++ F) ++ E).
-      eapply wf_typ_subst_cb...
-      constructor.
-      simpl. fsetdec.
-  - Case "wf_typ_all".
-    pick fresh Y and apply wf_typ_all...
-    + SCase "T2".
-      unfold open_ct in *...
-      rewrite subst_ct_open_tt_var...
-      rewrite_env (map (subst_cb Z C) ([(Y, bind_sub T1)] ++ F) ++ E).
-      eapply wf_typ_subst_cb...
-Qed.
+(* Lemma wf_typ_subst_cb : forall F Q E Z C T, *)
+(*   wf_typ (F ++ [(Z, bind_typ Q)] ++ E) T -> *)
+(*   (** NOTE here that P needs to be well formed in both the + and - environments, *)
+(*       as we're substituting in both places. *) *)
+(*   wf_cset E C -> *)
+(*   ok (map (subst_cb Z C) F ++ E) -> *)
+(*   ok (F ++ [(Z, bind_typ Q)] ++ E) -> *)
+(*   wf_typ (map (subst_cb Z C) F ++ E) (subst_ct Z C T) *)
+(* with wf_pretyp_subst_cb : forall F Q E Z C T, *)
+(*   wf_pretyp (F ++ [(Z, bind_typ Q)] ++ E) T -> *)
+(*   wf_cset E C -> *)
+(*   ok (map (subst_cb Z C) F ++ E) -> *)
+(*   ok (F ++ [(Z, bind_typ Q)] ++ E) -> *)
+(*   wf_pretyp (map (subst_cb Z C) F ++ E) (subst_cpt Z C T). *)
+(* Proof with simpl_env; eauto using wf_typ_weaken_head, type_from_wf_typ, wf_cset_subst_tb, *)
+(*     capt_from_wf_cset. *)
+(* ------ *)
+(*   intros F Q E Z C T HwfT HwfC Hok HokZ. *)
+(*   remember (F ++ [(Z, bind_typ Q)] ++ E). *)
+(*   generalize dependent F. *)
+(*   induction HwfT; intros F EQF Hok; subst; simpl subst_ct... *)
+(*   - Case "wf_typ_var". *)
+(*       binds_cases H... *)
+(*       apply (wf_typ_var (subst_ct Z C U))... *)
+(*   - Case "wf_typ_capt". *)
+(*     constructor... *)
+(*     apply wf_cset_over_subst with (Q := Q)... *)
+(* ------ *)
+(*   intros F Q E Z C T HwfT HwfC Hok HokZ. *)
+(*   remember (F ++ [(Z, bind_typ Q)] ++ E). *)
+(*   generalize dependent F. *)
+(*   induction HwfT; intros F EQF Hok; subst; simpl subst_ct. *)
+(*   - constructor. *)
+(*   - Case "wf_typ_arrow". *)
+(*     pick fresh Y and apply wf_typ_arrow... *)
+(*     + SCase "T2". *)
+(*       unfold open_ct in *... *)
+(*       rewrite <- subst_ct_open_ct_rec... *)
+(*       rewrite_env (map (subst_cb Z C) ([(Y, bind_typ T1)] ++ F) ++ E). *)
+(*       eapply wf_typ_subst_cb... *)
+(*       constructor. *)
+(*       simpl. fsetdec. *)
+(*   - Case "wf_typ_all". *)
+(*     pick fresh Y and apply wf_typ_all... *)
+(*     + SCase "T2". *)
+(*       unfold open_ct in *... *)
+(*       rewrite subst_ct_open_tt_var... *)
+(*       rewrite_env (map (subst_cb Z C) ([(Y, bind_sub T1)] ++ F) ++ E). *)
+(*       eapply wf_typ_subst_cb... *)
+(* Qed. *)
 
-Lemma wf_typ_open_capt : forall E C T1 T2,
-  ok E ->
-  wf_pretyp E (typ_arrow T1 T2) ->
-  wf_cset E C ->
-  wf_typ E (open_ct T2 C).
-Proof with simpl_env; eauto.
-  intros E U T1 T2 O WA WC.
-  inversion WA; subst.
-  pick fresh X.
-  rewrite (subst_ct_intro X)...
-  (** Needs new lemmas for opening a type with a capture set;
-      probably wf_typ_subst_eb and subst_ct_intro X *)
-  rewrite_env (map (subst_cb X U) empty ++ E).
-  apply wf_typ_subst_cb with (Q := T1)...
-Qed.
+(* Lemma wf_typ_open_capt : forall E C T1 T2, *)
+(*   ok E -> *)
+(*   wf_pretyp E (typ_arrow T1 T2) -> *)
+(*   wf_cset E C -> *)
+(*   wf_typ E (open_ct T2 C). *)
+(* Proof with simpl_env; eauto. *)
+(*   intros E U T1 T2 O WA WC. *)
+(*   inversion WA; subst. *)
+(*   pick fresh X. *)
+(*   rewrite (subst_ct_intro X)... *)
+(*   (** Needs new lemmas for opening a type with a capture set; *)
+(*       probably wf_typ_subst_eb and subst_ct_intro X *) *)
+(*   rewrite_env (map (subst_cb X U) empty ++ E). *)
+(*   apply wf_typ_subst_cb with (Q := T1)... *)
+(* Qed. *)
 
 
 (* ********************************************************************** *)
@@ -542,35 +626,49 @@ Hint Resolve ok_from_wf_env : core.
 Lemma wf_typ_from_binds_typ : forall x U E,
   wf_env E ->
   binds x (bind_typ U) E ->
-  wf_typ E U.
+  wf_typ_in E U.
 Proof with eauto using wf_typ_weaken_head.
   intros x U E Hwf Hbinds.
   (* remember m; generalize dependent m. *)
+  unfold wf_typ_in.
   induction Hwf; binds_cases Hbinds...
-  inversion H3; subst...
+  + eapply wf_typ_weaken_head...
+    all : simpl; fsetdec.
+  + eapply wf_typ_weaken_head...
+    all : simpl; fsetdec.
+  + inversion H3; subst...
+    eapply wf_typ_weaken_head...
+    all : simpl; fsetdec.
 Qed.
 
 Lemma wf_typ_from_binds_sub : forall x U E,
   wf_env E ->
   binds x (bind_sub U) E ->
-  wf_typ E U.
+  wf_typ_in E U.
 Proof with eauto using wf_typ_weaken_head.
   intros x U E Hwf Hbinds.
   (* remember m; generalize dependent m. *)
+  unfold wf_typ_in.
   induction Hwf; binds_cases Hbinds...
-  inversion H3; subst...
+  + eapply wf_typ_weaken_head...
+    all : simpl; fsetdec.
+  + inversion H3; subst...
+    eapply wf_typ_weaken_head...
+    all : simpl; fsetdec.
+  + eapply wf_typ_weaken_head...
+    all : simpl; fsetdec.
 Qed.
 
 Lemma wf_typ_from_wf_env_typ : forall x T E,
   wf_env ([(x, bind_typ T)] ++ E) ->
-  wf_typ E T.
+  wf_typ_in E T.
 Proof.
   intros x T E H. inversion H; auto.
 Qed.
 
 Lemma wf_typ_from_wf_env_sub : forall x T E,
   wf_env ([(x, bind_sub T)] ++ E) ->
-  wf_typ E T.
+  wf_typ_in E T.
 Proof.
   intros x T E H. inversion H; auto.
 Qed.
@@ -581,32 +679,32 @@ Qed.
 (** These properties are analogous to the properties that we need to
     show for the subtyping and typing relations. *)
 
-Lemma wf_env_narrowing : forall V E F U X,
-  wf_env (F ++ [(X, bind_sub V)] ++ E) ->
-  wf_typ E U ->
-  wf_env (F ++ [(X, bind_sub U)] ++ E).
-Proof with eauto 6 using wf_typ_narrowing.
-  induction F; intros U X Wf_env Wf;
-    inversion Wf_env; subst; simpl_env in *...
-Qed.
+(* Lemma wf_env_narrowing : forall V E F U X, *)
+(*   wf_env (F ++ [(X, bind_sub V)] ++ E) -> *)
+(*   wf_typ_in E U -> *)
+(*   wf_env (F ++ [(X, bind_sub U)] ++ E). *)
+(* Proof with eauto 6 using wf_typ_narrowing. *)
+(*   induction F; intros U X Wf_env Wf; *)
+(*     inversion Wf_env; subst; simpl_env in *... *)
+(* Qed. *)
 
-Lemma wf_env_narrowing_typ : forall V E F U X,
-  wf_env (F ++ [(X, bind_typ V)] ++ E) ->
-  wf_typ E U ->
-  wf_env (F ++ [(X, bind_typ U)] ++ E).
-Proof with eauto 6 using wf_typ_narrowing_typ, wf_cset_narrowing_typ.
-  induction F; intros U X Wf_env Wf;
-    inversion Wf_env; subst; simpl_env in *...
-Qed.
+(* Lemma wf_env_narrowing_typ : forall V E F U X, *)
+(*   wf_env (F ++ [(X, bind_typ V)] ++ E) -> *)
+(*   wf_typ E U -> *)
+(*   wf_env (F ++ [(X, bind_typ U)] ++ E). *)
+(* Proof with eauto 6 using wf_typ_narrowing_typ, wf_cset_narrowing_typ. *)
+(*   induction F; intros U X Wf_env Wf; *)
+(*     inversion Wf_env; subst; simpl_env in *... *)
+(* Qed. *)
 
-Lemma wf_env_subst_tb : forall Q Z P E F,
-  wf_env (F ++ [(Z, bind_sub Q)] ++ E) ->
-  wf_typ E P ->
-  wf_env (map (subst_tb Z P) F ++ E).
-Proof with eauto 6 using wf_typ_subst_tb.
-  induction F; intros Wf_env WP; simpl_env;
-    inversion Wf_env; simpl_env in *; simpl subst_tb...
-Qed.
+(* Lemma wf_env_subst_tb : forall Q Z P E F, *)
+(*   wf_env (F ++ [(Z, bind_sub Q)] ++ E) -> *)
+(*   wf_typ E P -> *)
+(*   wf_env (map (subst_tb Z P) F ++ E). *)
+(* Proof with eauto 6 using wf_typ_subst_tb. *)
+(*   induction F; intros Wf_env WP; simpl_env; *)
+(*     inversion Wf_env; simpl_env in *; simpl subst_tb... *)
+(* Qed. *)
 
 Lemma wf_env_inv : forall F Z b E,
   wf_env (F ++ [(Z, b)] ++ E) ->
@@ -631,14 +729,14 @@ with notin_fv_tpt_open_tpt_rec : forall k (Y X : atom) T,
 Proof.
 ------
   intros k Y X T. unfold open_tt.
-  generalize k. 
+  generalize k.
   induction T; simpl; intros k0 Fr; notin_simpl; try apply notin_union; eauto.
 ------
   intros k Y X T. unfold open_tt.
-  generalize k. 
+  generalize k.
   induction T; simpl; intros k0 Fr; notin_simpl; try apply notin_union; eauto.
 Qed.
- 
+
 
 Local Lemma notin_fv_tt_open_tt : forall (Y X : atom) T,
   X `notin` fv_tt (open_tt T Y) ->
@@ -659,10 +757,10 @@ with notin_fv_tt_open_ept_rec : forall (Y X : atom) T k,
   X `notin` fv_ept T.
 Proof.
 ------
-  intros Y X T. unfold open_tt_rec. 
+  intros Y X T. unfold open_tt_rec.
   induction T; simpl; intros k Fr; notin_simpl; try apply notin_union; eauto.
 ------
-  intros Y X T. unfold open_tt_rec. 
+  intros Y X T. unfold open_tt_rec.
   induction T; simpl; intros k Fr; notin_simpl; try apply notin_union; eauto.
 Qed.
 
@@ -673,7 +771,7 @@ with notin_fv_tt_open_ept : forall (Y X : atom) T,
   X `notin` fv_ept (open_tpt T Y) ->
   X `notin` fv_ept T.
 Proof with eauto.
-  intros. apply notin_fv_tt_open_et_rec with (k := 0) (Y := Y)... 
+  intros. apply notin_fv_tt_open_et_rec with (k := 0) (Y := Y)...
   intros. apply notin_fv_tt_open_ept_rec with (k := 0) (Y := Y)...
 Qed.
 
@@ -714,7 +812,7 @@ with notin_fv_cpt_open_tpt : forall (X : atom) T C,
   X `notin` fv_tpt (open_cpt T C) ->
   X `notin` fv_tpt T.
 Proof with eauto.
-  intros. apply notin_fv_ct_open_tt_rec with (k := 0) (C := C)... 
+  intros. apply notin_fv_ct_open_tt_rec with (k := 0) (C := C)...
   intros. apply notin_fv_cpt_open_tpt_rec with (k := 0) (C := C)...
 Qed.
 
@@ -728,8 +826,8 @@ Proof with auto.
   cset_split; destruct C eqn:HC; destruct c eqn:Hc...
 Qed.
 
-(* revert H. 
-    unfold fv_cset. unfold open_cset. 
+(* revert H.
+    unfold fv_cset. unfold open_cset.
     cset_split; destruct C eqn:HC; destruct c eqn:Hcd...
     admit.
      *)
@@ -745,7 +843,7 @@ Proof with auto.
 ------
   intros X T C.
   induction T ; simpl ; intros k H Fr ; try apply notin_union; eauto.
-  - apply notin_fv_open_cset with (k := k) (c := C)...    
+  - apply notin_fv_open_cset with (k := k) (c := C)...
   - apply notin_fv_ct_open_ept_rec with (C := C) (k := k)...
 ------
     intros X T C.
@@ -765,7 +863,7 @@ with notin_fv_ct_open_ept : forall (X : atom) T C,
   X `notin` fv_ept (open_cpt T C) ->
   X `notin` fv_ept T.
 Proof with auto.
-  intros. apply notin_fv_ct_open_et_rec with (k := 0) (C := C)... 
+  intros. apply notin_fv_ct_open_et_rec with (k := 0) (C := C)...
   intros. apply notin_fv_ct_open_ept_rec with (k := 0) (C := C)...
 Qed.
 
@@ -779,7 +877,7 @@ with notin_fv_ct_open_cpt_rec : forall (Y X : atom) T k,
   X `notin` fv_ept T.
 Proof with eauto*.
 ------
-  intros Y X T. 
+  intros Y X T.
   induction T ; simpl ; intros k H Fr ; try apply notin_union; eauto.
   - apply notin_fv_open_cset with (k := k) (c := Y)...
     discriminate.
@@ -802,7 +900,7 @@ with notin_fv_ct_open_cpt : forall (Y X : atom) T,
   X <> Y ->
   X `notin` fv_ept T.
 Proof with eauto*.
-  intros. apply notin_fv_ct_open_ct_rec with (k := 0) (Y := Y)... 
+  intros. apply notin_fv_ct_open_ct_rec with (k := 0) (Y := Y)...
   intros. apply notin_fv_ct_open_cpt_rec with (k := 0) (Y := Y)...
 Qed.
 
@@ -819,100 +917,100 @@ Proof with auto.
 Qed.
 
 
-Lemma notin_fv_wf_typ : forall E (X : atom) T,
-  wf_typ E T ->
-  X `notin` dom E ->
-  X `notin` (fv_tt T `union` fv_et T)
-with notin_fv_wf_pretyp : forall E (X : atom) T,
-  wf_pretyp E T ->
-  X `notin` dom E ->
-  X `notin` (fv_tpt T `union` fv_ept T).
-Proof with eauto.
-------
-  intros E X T Wf_typ.
-  induction Wf_typ; intros FrE; simpl...
-  (* Var *)
-  - assert (X0 `in` dom E) by (eapply binds_In; eauto)...
-  (* typ_cset *)
-  - specialize (notin_fv_wf_pretyp _ _ _ H0 FrE) as Wf.
-    inversion H;
-    destruct C.
-    + fsetdec.
-    + repeat apply notin_union; try fsetdec.
-    + contradict H2; discriminate.
-    + repeat apply notin_union; try fsetdec.
-      unfold fv_cset in *.
-      unfold allbound_typ in *.
-      unfold cset_fvar.
-      intro.
-      specialize (H1 X H4).
-      inversion H3; subst.
-      destruct H1.
-      assert (X `in` dom E). { eapply binds_In... }
-      contradiction.
-------
-  intros E X T Wf_typ.
-  induction Wf_typ; intros FrE; simpl...
-  (* typ_arrow *)
-  - pick fresh Y.
-    assert (Y `notin` L) by fsetdec.
-    assert (X `notin` dom ([(Y, bind_typ T1)] ++ E)). {
-      simpl_env. fsetdec.
-    }
-    specialize (H0 Y H1).
-    specialize (notin_fv_wf_typ _ _ _ H FrE) as Wf1.
-    specialize (notin_fv_wf_typ _ _ _ H0 H2) as Wf2.
-    notin_simpl.
-    repeat apply notin_union...
-    + apply notin_fv_ct_open_tt with (C := Y)...
-    + apply notin_fv_ct_open_et with (C := Y).
-      discriminate. intuition.
-  (* typ_all *)
-  - pick fresh Y.
-    assert (Y `notin` L) by fsetdec.
-    assert (X `notin` dom ([(Y, bind_typ T1)] ++ E)). {
-      simpl_env. fsetdec.
-    }
-    specialize (H0 Y H1).
-    specialize (notin_fv_wf_typ _ _ _ H FrE) as Wf1.
-    specialize (notin_fv_wf_typ _ _ _ H0 H2) as Wf2.
-    notin_simpl.
-    repeat apply notin_union...
-    + apply notin_fv_tt_open_tt with (Y := Y)...
-    + apply notin_fv_tt_open_et with (Y := Y)...
-Qed.
+(* Lemma notin_fv_wf_typ : forall E (X : atom) T, *)
+(*   wf_typ_in E T -> *)
+(*   X `notin` dom E -> *)
+(*   X `notin` (fv_tt T `union` fv_et T) *)
+(* with notin_fv_wf_pretyp : forall E (X : atom) T, *)
+(*   wf_pretyp_in E T -> *)
+(*   X `notin` dom E -> *)
+(*   X `notin` (fv_tpt T `union` fv_ept T). *)
+(* Proof with eauto. *)
+(* ------ *)
+(*   intros E X T Wf_typ. *)
+(*   induction Wf_typ; intros FrE; simpl... *)
+(*   (* Var *) *)
+(*   - assert (X0 `in` dom E) by (eapply binds_In; eauto)... *)
+(*   (* typ_cset *) *)
+(*   - specialize (notin_fv_wf_pretyp _ _ _ H0 FrE) as Wf. *)
+(*     inversion H; *)
+(*     destruct C. *)
+(*     + fsetdec. *)
+(*     + repeat apply notin_union; try fsetdec. *)
+(*     + contradict H2; discriminate. *)
+(*     + repeat apply notin_union; try fsetdec. *)
+(*       unfold fv_cset in *. *)
+(*       unfold allbound_typ in *. *)
+(*       unfold cset_fvar. *)
+(*       intro. *)
+(*       specialize (H1 X H4). *)
+(*       inversion H3; subst. *)
+(*       destruct H1. *)
+(*       assert (X `in` dom E). { eapply binds_In... } *)
+(*       contradiction. *)
+(* ------ *)
+(*   intros E X T Wf_typ. *)
+(*   induction Wf_typ; intros FrE; simpl... *)
+(*   (* typ_arrow *) *)
+(*   - pick fresh Y. *)
+(*     assert (Y `notin` L) by fsetdec. *)
+(*     assert (X `notin` dom ([(Y, bind_typ T1)] ++ E)). { *)
+(*       simpl_env. fsetdec. *)
+(*     } *)
+(*     specialize (H0 Y H1). *)
+(*     specialize (notin_fv_wf_typ _ _ _ H FrE) as Wf1. *)
+(*     specialize (notin_fv_wf_typ _ _ _ H0 H2) as Wf2. *)
+(*     notin_simpl. *)
+(*     repeat apply notin_union... *)
+(*     + apply notin_fv_ct_open_tt with (C := Y)... *)
+(*     + apply notin_fv_ct_open_et with (C := Y). *)
+(*       discriminate. intuition. *)
+(*   (* typ_all *) *)
+(*   - pick fresh Y. *)
+(*     assert (Y `notin` L) by fsetdec. *)
+(*     assert (X `notin` dom ([(Y, bind_typ T1)] ++ E)). { *)
+(*       simpl_env. fsetdec. *)
+(*     } *)
+(*     specialize (H0 Y H1). *)
+(*     specialize (notin_fv_wf_typ _ _ _ H FrE) as Wf1. *)
+(*     specialize (notin_fv_wf_typ _ _ _ H0 H2) as Wf2. *)
+(*     notin_simpl. *)
+(*     repeat apply notin_union... *)
+(*     + apply notin_fv_tt_open_tt with (Y := Y)... *)
+(*     + apply notin_fv_tt_open_et with (Y := Y)... *)
+(* Qed. *)
 
-Lemma notin_fv_wf : forall E (X : atom) T,
-  wf_typ E T ->
-  X `notin` dom E ->
-  X `notin` fv_tt T.
-Proof with eauto.
-  intros E X T Wf_typ F.
-  assert (X `notin` (fv_tt T `union` fv_et T)). {
-    eapply notin_fv_wf_typ...
-  }
-  fsetdec.
-Qed.
+(* Lemma notin_fv_wf : forall E (X : atom) T, *)
+(*   wf_typ E T -> *)
+(*   X `notin` dom E -> *)
+(*   X `notin` fv_tt T. *)
+(* Proof with eauto. *)
+(*   intros E X T Wf_typ F. *)
+(*   assert (X `notin` (fv_tt T `union` fv_et T)). { *)
+(*     eapply notin_fv_wf_typ... *)
+(*   } *)
+(*   fsetdec. *)
+(* Qed. *)
 
-Lemma map_subst_tb_id : forall G Z P,
-  wf_env G ->
-  Z `notin` dom G ->
-  G = map (subst_tb Z P) G.
-Proof with auto.
-  intros G Z P H.
-  induction H; simpl; intros Fr; simpl_env...
-  rewrite <- IHwf_env...
-    rewrite <- subst_tt_fresh... eapply notin_fv_wf; eauto.
-  rewrite <- IHwf_env...
-    rewrite <- subst_tt_fresh... eapply notin_fv_wf; eauto.
-Qed.
+(* Lemma map_subst_tb_id : forall G Z P, *)
+(*   wf_env G -> *)
+(*   Z `notin` dom G -> *)
+(*   G = map (subst_tb Z P) G. *)
+(* Proof with auto. *)
+(*   intros G Z P H. *)
+(*   induction H; simpl; intros Fr; simpl_env... *)
+(*   rewrite <- IHwf_env... *)
+(*     rewrite <- subst_tt_fresh... eapply notin_fv_wf; eauto. *)
+(*   rewrite <- IHwf_env... *)
+(*     rewrite <- subst_tt_fresh... eapply notin_fv_wf; eauto. *)
+(* Qed. *)
 
 (* ********************************************************************** *)
 (** * #<a name="regularity"></a># Regularity of relations *)
 
 Lemma subcapt_regular : forall E C1 C2,
   subcapt E C1 C2 ->
-  wf_cset E C1 /\ wf_cset E C2.
+  wf_cset E (dom E) C1 /\ wf_cset E (dom E) C2.
 Proof with eauto*.
   intros. inversion H...
 Qed.
@@ -926,12 +1024,15 @@ Proof with eauto*.
   - pose proof (subcapt_regular _ _ _ H1) as [WFenv [_ WfC]]...
 Qed. *)
 
+Hint Unfold wf_typ_in : core.
+Hint Unfold wf_pretyp_in : core.
+
 Lemma sub_regular : forall E S T,
   sub E S T ->
-  wf_env E /\ wf_typ E S /\ wf_typ E T
+  wf_env E /\ wf_typ_in E S /\ wf_typ_in E T
 with sub_pre_regular : forall E S T,
   sub_pre E S T ->
-  wf_env E /\ wf_pretyp E S /\ wf_pretyp E T.
+  wf_env E /\ wf_pretyp_in E S /\ wf_pretyp_in E T.
 Proof with simpl_env; auto*.
 ------
   intros E S T H.
@@ -941,8 +1042,8 @@ Proof with simpl_env; auto*.
     repeat split...
     apply wf_typ_var with (U := U)...
   - Case "sub_capt".
-    assert (wf_cset E C1 /\ wf_cset E C2). { apply subcapt_regular... }
-    assert (wf_env E /\ wf_pretyp E P1 /\ wf_pretyp E P2). { apply sub_pre_regular... }
+    assert (wf_cset_in E C1 /\ wf_cset_in E C2). { apply subcapt_regular... }
+    assert (wf_env E /\ wf_pretyp_in E P1 /\ wf_pretyp_in E P2). { apply sub_pre_regular... }
     repeat split...
 ------
   intros E S T H.
@@ -951,33 +1052,36 @@ Proof with simpl_env; auto*.
   - Case  "sub_trans_arrow".
     pose proof (sub_regular E _ _ H).
     repeat split...
-    + (* S1 -> S2 wf *)
-      pick fresh Y and apply wf_typ_arrow...
-      assert (Y `notin` L) by fsetdec.
-      rewrite_env (empty ++ [(Y, bind_typ S1)] ++ E).
-      apply wf_typ_narrowing_typ with (C1 := T1)...
-      specialize (H0 Y H2).
-      pose proof (sub_regular _ _ _ H0)...
-    + (* T1 -> T2 wf *)
-      pick fresh Y and apply wf_typ_arrow...
-      assert (Y `notin` L) by fsetdec.
-      specialize (H0 Y H2).
-      pose proof (sub_regular _ _ _ H0)...
+    (* + (* S1 -> S2 wf *) *)
+    (*   pick fresh Y and apply wf_typ_arrow... *)
+    (*   assert (Y `notin` L) by fsetdec. *)
+    (*   rewrite_env (empty ++ [(Y, bind_typ S1)] ++ E). *)
+    (*   apply wf_typ_narrowing_typ with (C1 := T1)... *)
+    (*   specialize (H0 Y H2). *)
+    (*   pose proof (sub_regular _ _ _ H0)... *)
+    (*   replace (dom E `union` singleton Y) with (dom ([(Y, bind_typ T1)] ++ E))... *)
+    (*   simpl dom in *. *)
+    (* + (* T1 -> T2 wf *) *)
+    (*   pick fresh Y and apply wf_typ_arrow... *)
+    (*   assert (Y `notin` L) by fsetdec. *)
+    (*   specialize (H0 Y H2). *)
+    (*   pose proof (sub_regular _ _ _ H0)... *)
   - Case "sub_all".
     pose proof (sub_regular E _ _ H).
     repeat split...
-    SCase "Second of original three conjuncts".
-      pick fresh Y and apply wf_typ_all...
-      assert (Y `notin` L) by fsetdec.
-      specialize (H0 Y H2).
-      destruct (sub_regular _ _ _ H0) as [_ [Wf _]]...
-      rewrite_env (empty ++ [(Y, bind_sub S1)] ++ E).
-      apply (wf_typ_narrowing T1)...
-    SCase "Third of original three conjuncts".
-      pick fresh Y and apply wf_typ_all...
-      assert (Y `notin` L) by fsetdec.
-      specialize (H0 Y H2).
-      destruct (sub_regular _ _ _ H0) as [_ [_ Wf]]...
+    all : trivial.
+    (* SCase "Second of original three conjuncts". *)
+    (*   pick fresh Y and apply wf_typ_all... *)
+    (*   assert (Y `notin` L) by fsetdec. *)
+    (*   specialize (H0 Y H2). *)
+    (*   destruct (sub_regular _ _ _ H0) as [_ [Wf _]]... *)
+    (*   rewrite_env (empty ++ [(Y, bind_sub S1)] ++ E). *)
+    (*   apply (wf_typ_narrowing T1)... *)
+    (* SCase "Third of original three conjuncts". *)
+    (*   pick fresh Y and apply wf_typ_all... *)
+    (*   assert (Y `notin` L) by fsetdec. *)
+    (*   specialize (H0 Y H2). *)
+    (*   destruct (sub_regular _ _ _ H0) as [_ [_ Wf]]... *)
 Qed.
 
 Lemma cv_free_never_universal : forall e,
@@ -993,7 +1097,7 @@ Qed.
 Lemma cv_free_is_bvar_free : forall e,
   empty_cset_bvars (free_for_cv e).
 Proof with eauto using cv_free_never_universal.
-  intros. induction e... 
+  intros. induction e...
   - simpl; fnsetdec...
   - simpl; fnsetdec...
   - unfold empty_cset_bvars in *.
@@ -1101,20 +1205,21 @@ Proof with eauto*.
   split; intros; assert (x `in` (T1 `union` T2)) by fsetdec...
 Qed.
 
-Lemma wf_cset_over_union : forall E C1 C2,
+Lemma wf_cset_over_union : forall E A C1 C2,
   C1 <> cset_universal ->
   C2 <> cset_universal ->
-  wf_cset E (cset_union C1 C2) <->
-  wf_cset E C1 /\ wf_cset E C2.
+  wf_cset E A (cset_union C1 C2) <->
+  wf_cset E A C1 /\ wf_cset E A C2.
 Proof with eauto*.
   intros; split; intros; destruct C1 eqn:HC1;
                          destruct C2 eqn:HC2;
                          unfold cset_union in *...
   + inversion H1; subst...
-    apply empty_over_union in H5; inversion H5.
-    apply allbound_over_union in H4; inversion H4.
+    apply empty_over_union in H3; inversion H3.
+    apply allbound_over_union in H6; inversion H6.
     subst.
     split; constructor...
+    all : fsetdec.
   + destruct H1 as [Hwf1 Hwf2].
     inversion Hwf1; inversion Hwf2; subst...
     (** this should really be a lemma... *)
@@ -1123,6 +1228,7 @@ Proof with eauto*.
     unfold allbound_typ in *...
     intros.
     apply AtomSetFacts.union_iff in H2...
+    fsetdec.
 Qed.
 
 Lemma cset_references_fvar_over_union : forall C1 C2 x,
@@ -1141,7 +1247,7 @@ Proof with eauto*.
 Qed.
 
 Lemma free_for_cv_bound : forall E e (x : atom),
-  wf_cset E (free_for_cv e) ->
+  wf_cset_in E (free_for_cv e) ->
   cset_references_fvar x (free_for_cv e) ->
   exists T, binds x (bind_typ T) E.
 Proof with eauto using wf_cset_over_union, cv_free_never_universal.
@@ -1162,7 +1268,7 @@ Proof with eauto using cv_free_never_universal; eauto*.
   intros e.
   (** gah why doesn't eauto pick this up. *)
   pose proof (cv_free_never_universal).
-  induction e; try destruct (free_for_cv e) eqn:Hcve; 
+  induction e; try destruct (free_for_cv e) eqn:Hcve;
     subst; simpl; try rewrite Hcve; try constructor; try inversion IHe;
     try fsetdec; try fnsetdec.
   - unfold cset_union in *;
@@ -1172,21 +1278,27 @@ Proof with eauto using cv_free_never_universal; eauto*.
     constructor; try fsetdec; try fnsetdec...
 Qed.
 
+Hint Extern 10 (AtomSet.F.Subset _ _) =>
+  idtac "go fsetdec go" ; fsetdec
+: core.
+
 (** This should be easily true: free variables
     are all bound if a term has a type.... *)
 Lemma typing_cv : forall E e T,
   typing E e T ->
-  wf_cset E (free_for_cv e).
+  wf_cset_in E (free_for_cv e).
 Proof with eauto using cv_free_never_universal, wf_cset_over_union; eauto*.
   intros E e T Htyp.
   induction Htyp; simpl...
   (** TODO: merge the abs/t-abs case somehow (maybe a match to decide what
       gets posed? )*)
-  - simpl. constructor.
+  - pose proof (binds_In _ _ _ _ H0).
+    simpl. constructor...
     unfold allbound_typ. intros.
     assert (x = x0) by fsetdec.
     subst. exists X...
-  - simpl. constructor.
+  - pose proof (binds_In _ _ _ _ H0).
+    simpl. constructor...
     unfold allbound_typ. intros.
     assert (x = x0) by fsetdec.
     subst. exists (typ_capt C P)...
@@ -1208,15 +1320,19 @@ Proof with eauto using cv_free_never_universal, wf_cset_over_union; eauto*.
     unfold open_ee in *.
     inversion H0; subst...
     inversion H3; subst...
-    rewrite <- H6 in H10. inversion H10; subst...
+    rewrite <- H6 in H11. inversion H11; subst...
     assert (t0 = {}N) by fnsetdec; subst...
     constructor...
+    2: {
+      simpl dom in *.
+      fsetdec.
+    }
     unfold allbound_typ in *.
     intros.
     destruct (x == y)...
     assert (x `in` fvars) by fsetdec.
-    specialize (H8 x H9).
-    inversion H8 as [T Hbinds]; subst...
+    specialize (H7 x H9).
+    inversion H7 as [T Hbinds]; subst...
     exists T.
     binds_cases Hbinds...
   - simpl...
@@ -1240,128 +1356,135 @@ Proof with eauto using cv_free_never_universal, wf_cset_over_union; eauto*.
     unfold open_te in *.
     inversion H0; subst...
     inversion H3; subst...
-    rewrite <- H6 in H10. inversion H10; subst...
+    rewrite <- H6 in H11. inversion H11; subst...
     assert (t0 = {}N) by fnsetdec; subst...
     constructor...
     unfold allbound_typ in *.
     intros.
     destruct (x == y)...
     assert (x `in` fvars) by fsetdec.
-    specialize (H8 x H9).
-    inversion H8 as [T Hbinds]; subst...
+    specialize (H7 x H9).
+    inversion H7 as [T Hbinds]; subst...
     exists T.
     binds_cases Hbinds...
+    simpl dom in *.
+    fsetdec.
 Qed.
 
 (** The things that the cv relation returns are all well-formed,
     assuming the type is well formed... *)
 Lemma cv_wf : forall E T C,
   cv E T C ->
-  wf_cset E C.
+  wf_cset_in E C.
 Proof with simpl_env; eauto*.
   intros E T C HC.
   induction HC; intros; subst.
-  * apply wf_cset_weaken_head...
-  * apply wf_cset_weaken_head...
-  * assumption.
-Qed.
+  all : admit.
+Admitted.
+(*   * apply wf_cset_weaken_head... *)
+(*   * apply wf_cset_weaken_head... *)
+(*   * assumption. *)
+(* Qed. *)
 
 Lemma typing_regular : forall E e T,
   typing E e T ->
-  wf_env E /\ expr e /\ wf_typ E T.
+  wf_env E /\ expr e /\ wf_typ_in E T.
 Proof with simpl_env; auto*.
-  intros E e T H. induction H...
-  (* typing rule: x : T \in E --> E |- x : {x} T *)
+  intros E e T H.
+  admit.
+  (* induction H... *)
+  (* (* typing rule: x : T \in E --> E |- x : {x} T *) *)
 
-  (* typing_var_tvar  *)
-  - repeat split...
-    apply wf_typ_from_binds_typ with (x := x)...
-  (* typing_var_poly  *)
-  - repeat split...
-    assert (wf_typ E (typ_capt C P)). {
-      apply wf_typ_from_binds_typ with (x := x)...
-    }
-    subst.
-    inversion H1; subst.    
-    constructor...
-    constructor.
-    unfold allbound_typ. intros.
-    assert (x0 = x) by fsetdec.
-    subst; eauto.
-  (* typing rule: (\x e) has type fv((\x e)) T1 -> T2 *)
-  - pick fresh y; assert (y `notin` L) by fsetdec...
-    specialize (H0 y H1) as H3; inversion H3 as [Henv [Hexpr Hwf]]...
-    repeat split...
-    (* wf_env *)
-    + inversion Henv...
-    (* expr *)
-    + pick fresh x and apply expr_abs.
-      * eauto using type_from_wf_typ, wf_typ_from_wf_env_typ.
-      * destruct (H0 x)...
-    (* wf_typ *)
-    + constructor...
-    assert (typing E (exp_abs V e1) (typ_capt (free_for_cv e1) (typ_arrow V T1))). { 
-      apply typing_abs with (L := L). apply H. 
-    }
-    apply typing_cv with (e := (exp_abs V e1)) (T := (typ_capt (free_for_cv e1) (typ_arrow V T1)))...      
-    pick fresh x and apply wf_typ_arrow...
-    * eauto using type_from_wf_typ, wf_typ_from_wf_env_typ.
-    * destruct (H0 x)...
-  (* typing rule: app poly *)  
-  - destruct IHtyping1 as [Hwf [Hexpr1 HwfF]].
-    inversion HwfF; subst...
-    destruct (sub_regular _ _ _ H1) as [_ [Wf1 Wf2]].
-    inversion Wf2; subst...
-    (** why are these two cases the same... *)
-    {
-      repeat split...
-      + constructor...
-        apply capt_from_wf_cset with (E := E).
-        unshelve epose proof (subcapt_regular E C Cv _) as [Hfinish _]...
-      + unshelve epose proof (wf_typ_open_capt E C X T2 _ _ _)...
-        unshelve epose proof (subcapt_regular E C Cv _) as [Hfinish _]...
-    }
-    {
-      repeat split...
-      + constructor...
-        apply capt_from_wf_cset with (E := E).
-        unshelve epose proof (subcapt_regular E C Cv _) as [Hfinish _]...
-      + unshelve epose proof (wf_typ_open_capt E C (typ_capt C0 P) T2 _ _ _)...
-        unshelve epose proof (subcapt_regular E C Cv _) as [Hfinish _]...
-    }
-  (* typing rule: (/\ X e) has type fv(/\ X e) X <: T1 -> T2 *)
-  - pick fresh Y. assert (Y `notin` L) by fsetdec...
-    specialize (H0 Y H1) as H3; inversion H3...
-    repeat split...
-    (* wf_env *)
-    + inversion H2...
-    (* expr *)
-    + econstructor...
-      * apply type_from_wf_typ with (E := E).
-        apply wf_typ_from_wf_env_sub with (x := Y)...
-      * instantiate (1 := L). intros...
-        specialize (H0 X H5) as H8...
-    (* wf_typ *)
-    + constructor...
-      assert (typing E (exp_tabs V e1) (typ_capt (free_for_cv e1) (typ_all V T1))). { 
-        apply typing_tabs with (L := L). apply H. 
-      }
-      apply typing_cv with (e := (exp_tabs V e1)) (T := (typ_capt (free_for_cv e1) (typ_all V T1)))...
-      pick fresh X and apply wf_typ_all...
-      * eauto using type_from_wf_typ, wf_typ_from_wf_env_sub.
-      * destruct (H0 X)...
-  (* typing rule: t-app *)
-  - repeat split...
-    constructor...
-    pose proof (sub_regular E T T1 H0).
-    apply type_from_wf_typ with (E := E)...
-    destruct (sub_regular _ _ _ H0) as [R1 [R2 R3]].
-    apply wf_typ_open with (T1 := T1)...
-    inversion IHtyping as [Henv [Hexpr Hwf_capt]].
-    inversion Hwf_capt; subst...
-  - repeat split...
-    pose proof (sub_regular E S T H0)...
-Qed.
+  (* (* typing_var_tvar  *) *)
+  (* - repeat split... *)
+  (*   apply wf_typ_from_binds_typ with (x := x)... *)
+  (* (* typing_var_poly  *) *)
+  (* - repeat split... *)
+  (*   assert (wf_typ E (typ_capt C P)). { *)
+  (*     apply wf_typ_from_binds_typ with (x := x)... *)
+  (*   } *)
+  (*   subst. *)
+  (*   inversion H1; subst. *)
+  (*   constructor... *)
+  (*   constructor. *)
+  (*   unfold allbound_typ. intros. *)
+  (*   assert (x0 = x) by fsetdec. *)
+  (*   subst; eauto. *)
+  (* (* typing rule: (\x e) has type fv((\x e)) T1 -> T2 *) *)
+  (* - pick fresh y; assert (y `notin` L) by fsetdec... *)
+  (*   specialize (H0 y H1) as H3; inversion H3 as [Henv [Hexpr Hwf]]... *)
+  (*   repeat split... *)
+  (*   (* wf_env *) *)
+  (*   + inversion Henv... *)
+  (*   (* expr *) *)
+  (*   + pick fresh x and apply expr_abs. *)
+  (*     * eauto using type_from_wf_typ, wf_typ_from_wf_env_typ. *)
+  (*     * destruct (H0 x)... *)
+  (*   (* wf_typ *) *)
+  (*   + constructor... *)
+  (*   assert (typing E (exp_abs V e1) (typ_capt (free_for_cv e1) (typ_arrow V T1))). { *)
+  (*     apply typing_abs with (L := L). apply H. *)
+  (*   } *)
+  (*   apply typing_cv with (e := (exp_abs V e1)) (T := (typ_capt (free_for_cv e1) (typ_arrow V T1)))... *)
+  (*   pick fresh x and apply wf_typ_arrow... *)
+  (*   * eauto using type_from_wf_typ, wf_typ_from_wf_env_typ. *)
+  (*   * destruct (H0 x)... *)
+  (* (* typing rule: app poly *) *)
+  (* - destruct IHtyping1 as [Hwf [Hexpr1 HwfF]]. *)
+  (*   inversion HwfF; subst... *)
+  (*   destruct (sub_regular _ _ _ H1) as [_ [Wf1 Wf2]]. *)
+  (*   inversion Wf2; subst... *)
+  (*   (** why are these two cases the same... *) *)
+  (*   { *)
+  (*     repeat split... *)
+  (*     + constructor... *)
+  (*       apply capt_from_wf_cset with (E := E). *)
+  (*       unshelve epose proof (subcapt_regular E C Cv _) as [Hfinish _]... *)
+  (*     + unshelve epose proof (wf_typ_open_capt E C X T2 _ _ _)... *)
+  (*       unshelve epose proof (subcapt_regular E C Cv _) as [Hfinish _]... *)
+  (*   } *)
+  (*   { *)
+  (*     repeat split... *)
+  (*     + constructor... *)
+  (*       apply capt_from_wf_cset with (E := E). *)
+  (*       unshelve epose proof (subcapt_regular E C Cv _) as [Hfinish _]... *)
+  (*     + unshelve epose proof (wf_typ_open_capt E C (typ_capt C0 P) T2 _ _ _)... *)
+  (*       unshelve epose proof (subcapt_regular E C Cv _) as [Hfinish _]... *)
+  (*   } *)
+  (* (* typing rule: (/\ X e) has type fv(/\ X e) X <: T1 -> T2 *) *)
+  (* - pick fresh Y. assert (Y `notin` L) by fsetdec... *)
+  (*   specialize (H0 Y H1) as H3; inversion H3... *)
+  (*   repeat split... *)
+  (*   (* wf_env *) *)
+  (*   + inversion H2... *)
+  (*   (* expr *) *)
+  (*   + econstructor... *)
+  (*     * apply type_from_wf_typ with (E := E). *)
+  (*       apply wf_typ_from_wf_env_sub with (x := Y)... *)
+  (*     * instantiate (1 := L). intros... *)
+  (*       specialize (H0 X H5) as H8... *)
+  (*   (* wf_typ *) *)
+  (*   + constructor... *)
+  (*     assert (typing E (exp_tabs V e1) (typ_capt (free_for_cv e1) (typ_all V T1))). { *)
+  (*       apply typing_tabs with (L := L). apply H. *)
+  (*     } *)
+  (*     apply typing_cv with (e := (exp_tabs V e1)) (T := (typ_capt (free_for_cv e1) (typ_all V T1)))... *)
+  (*     pick fresh X and apply wf_typ_all... *)
+  (*     * eauto using type_from_wf_typ, wf_typ_from_wf_env_sub. *)
+  (*     * destruct (H0 X)... *)
+  (* (* typing rule: t-app *) *)
+  (* - repeat split... *)
+  (*   constructor... *)
+  (*   pose proof (sub_regular E T T1 H0). *)
+  (*   apply type_from_wf_typ with (E := E)... *)
+  (*   destruct (sub_regular _ _ _ H0) as [R1 [R2 R3]]. *)
+  (*   apply wf_typ_open with (T1 := T1)... *)
+  (*   inversion IHtyping as [Henv [Hexpr Hwf_capt]]. *)
+  (*   inversion Hwf_capt; subst... *)
+  (* - repeat split... *)
+  (*   pose proof (sub_regular E S T H0)... *)
+(* Qed. *)
+Admitted.
 
 Lemma value_regular : forall e,
   value e ->
@@ -1375,13 +1498,14 @@ Lemma red_regular : forall e e',
   expr e /\ expr e'.
 Proof with auto*.
   intros e e' H.
-  induction H; assert(J := value_regular); split...
-  - Case "red_abs".
-    inversion H. pick fresh y. rewrite (subst_ee_intro y)...
-  - Case "red_tabs".
-    inversion H. pick fresh Y. rewrite (subst_te_intro Y)...
-Qed.
-
+  admit.
+(*   induction H; assert(J := value_regular); split... *)
+(*   - Case "red_abs". *)
+(*     inversion H. pick fresh y. rewrite (subst_ee_intro y)... *)
+(*   - Case "red_tabs". *)
+(*     inversion H. pick fresh Y. rewrite (subst_te_intro Y)... *)
+(* Qed. *)
+Admitted.
 
 (* *********************************************************************** *)
 (** * #<a name="auto"></a># Automation *)
