Fsub_Soundness.v
@@ -14,13 +14,89 @@
 
 Require Export Fsub_Lemmas.
 
+(* Require Import Atom. *)
 
 (* ********************************************************************** *)
 (** * #<a name="subtyping"></a># Properties of subtyping *)
 
+Lemma subcapt_reflexivity : forall E A C,
+  wf_env E ->
+  (* We need as a precondition that C is locally closed! *)
+  wf_cset E A C ->
+  AtomSet.F.Subset A (dom E) ->
+  subcapt E C C.
+Proof with auto.
+  intros *.
+  intros Ok Closed Hsubset.
+  destruct C...
+  + constructor.
+    constructor.
+  + assert (t0 = {}N). { inversion Closed... }
+    subst.
+    apply subcapt_set...
+    3: {
+      unfold AtomSet.F.For_all. intros.
+      apply captures_in...
+    }
+    all : admit.
+Admitted.
+(* Qed. *)
+
+Set Nested Proofs Allowed.
+Lemma come_on : forall E Ap Am Ap' Am' T,
+  wf_typ E Ap Am T ->
+  ok E ->
+  AtomSet.F.Subset Ap Ap' ->
+  AtomSet.F.Subset Am Am' ->
+  wf_typ E Ap' Am' T.
+Proof.
+  intros.
+  rewrite_env (empty ++ empty ++ E).
+  rewrite_env (empty ++ E) in H.
+  eapply wf_typ_weakening; eauto.
+Qed.
+
+Lemma sub_reflexivity : forall E Ap Am T,
+  wf_env E ->
+  wf_typ E Ap Am T ->
+  AtomSet.F.Subset Ap (dom E) ->
+  AtomSet.F.Subset Am (dom E) ->
+  sub E T T
+with sub_pre_reflexivity : forall E Ap Am T,
+  wf_env E ->
+  wf_pretyp E Ap Am T ->
+  AtomSet.F.Subset Ap (dom E) ->
+  AtomSet.F.Subset Am (dom E) ->
+  sub_pre E T T.
+Proof with eauto using subcapt_reflexivity, come_on.
+------
+  intros *.
+  intros Ok Wf HsubsetAp HsubsetAm.
+  induction Wf.
+  (* eauto and econstructor is still broken... hence we need to proof this manually *)
+  - apply sub_refl_tvar.
+    auto.
+    eapply wf_typ_var with (U := U)...
+  - apply sub_capt...
+------
+  intros *.
+  intros Ok Wf HsubsetAp HsubsetAm.
+  induction Wf.
+  - apply sub_top...
+  - apply sub_arrow with (L := L `union` dom E)...
+    + apply wf_typ_arrow with (L := L `union` dom E)...
+    + apply wf_typ_arrow with (L := L `union` dom E)...
+    + intros; eapply sub_reflexivity; simpl dom...
+  - apply sub_all with (L := L `union` dom E)...
+    + apply wf_typ_all with (L := L `union` dom E)...
+    + apply wf_typ_all with (L := L `union` dom E)...
+    + intros; eapply sub_reflexivity; simpl dom...
+Qed.
+
 
 (* ********************************************************************** *)
 (** ** Weakening (2) *)
+
 Require Import Coq.Program.Equality.
 
 Lemma cv_regular : forall E T C,
@@ -29,7 +105,7 @@ Lemma cv_regular : forall E T C,
 Proof with eauto*.
   intros. induction H...
   * repeat split...
-    destruct IHcv as [_ [_ HC]]. 
+    destruct IHcv as [_ [_ HC]].
     rewrite_env (empty ++ [(X, bind_sub T)] ++ E).
     apply wf_cset_weakening...
   * repeat split...
@@ -45,7 +121,7 @@ Lemma cv_weakening_head : forall E F T C,
 Proof with eauto using cv_regular.
   intros E F T C Hcv.
   induction F...
-  
+
   intros; destruct a; simpl_env in *...
   pose proof (cv_regular E T C Hcv).
   assert (wf_env (F ++ E)).
@@ -88,7 +164,7 @@ Proof with eauto using cv_regular, cv_weakening_head.
     destruct (Y == X); subst...
     {
       rewrite x in *.
-      inversion x; subst...     
+      inversion x; subst...
       specialize (IHHcv E G).
       constructor...
       apply IHHcv...
@@ -96,7 +172,7 @@ Proof with eauto using cv_regular, cv_weakening_head.
     }
     {
       rewrite x in *.
-      inversion x; subst...     
+      inversion x; subst...
       specialize (IHHcv E G).
       constructor...
       apply IHHcv...
@@ -281,7 +357,7 @@ Proof with eauto.
   - inversion H3...
   - simpl_env in *.
     binds_cases H3...
-    + assert (wf_typ E a0) by 
+    + assert (wf_typ E a0) by
         (apply wf_typ_var with (U := U); eauto).
       specialize (IHE a0 H6 H2) as [C' H'].
       inversion H'; subst...
@@ -312,7 +388,7 @@ Proof with eauto.
       apply cv_env_irrel...
       rewrite dom_concat in *.
       rewrite dom_single in *.
-      fsetdec.    
+      fsetdec.
 Qed.
 
 Lemma wf_env_weaken_head : forall E F,
@@ -336,7 +412,7 @@ Proof with eauto*.
     inversion H1; inversion H2; subst...
   }
   {
-    (*contradiction *) 
+    (*contradiction *)
     inversion H0.
   }
   {
@@ -349,7 +425,7 @@ Proof with eauto*.
     inversion H2...
   }
   {
-    inversion H0. 
+    inversion H0.
   }
   {
     destruct a as [a' B].
@@ -456,9 +532,9 @@ Lemma sub_implies_subcapt : forall E S T C D,
 Proof with eauto using subcapt_reflexivity, cv_weakening_head.
   intros E S T C D Hsub WfC WfD HcvC HcvD.
 
-  induction Hsub; destruct C; destruct D; try solve [inversion HcvC; inversion HcvD; eauto].  
+  induction Hsub; destruct C; destruct D; try solve [inversion HcvC; inversion HcvD; eauto].
   - pose proof (cv_unique _ _ _ _ H H0 HcvC HcvD) as Eq; inversion Eq...
-  - pose proof (cv_unique _ _ _ _ H H0 HcvC HcvD) as Eq; inversion Eq...  
+  - pose proof (cv_unique _ _ _ _ H H0 HcvC HcvD) as Eq; inversion Eq...
   - pose proof (cv_unique _ _ _ _ H H0 HcvC HcvD) as Eq; inversion Eq...
   - exfalso. admit.
     (* inversion HcvC; subst. inversion H1. inversion H. rewrite H4 in H2. inversion H2; subst. *)
@@ -469,9 +545,9 @@ Proof with eauto using subcapt_reflexivity, cv_weakening_head.
     + epose proof (cv_unique _ _ _ _ _ _ H3 H8) as Eq; inversion Eq...
     + assert (T0 = U) by admit. subst.
       inversion Hsub; subst.
-      * assert (cv ([(X, bind_sub X0)] ++ E0) X0 (cset_set t t0))...        
+      * assert (cv ([(X, bind_sub X0)] ++ E0) X0 (cset_set t t0))...
       * apply IHHsub...
-    + assert (T0 = U) by admit. subst.       
+    + assert (T0 = U) by admit. subst.
       apply IHHsub...
     + inversion H4; subst.
       * assert (T0 = U) by admit; subst...
@@ -573,12 +649,12 @@ Lemma captures_narrowing : forall F Z P Q E xs x,
 Proof with eauto using wf_cset_narrowing, wf_env_narrowing, cv_narrowing.
   intros F Z P Q E xs x Ok Sub H.
   remember (F ++ [(Z, bind_sub Q)] ++ E). generalize dependent F.
-  induction H; intros; subst...  
+  induction H; intros; subst...
   - assert (x <> Z). {
       unfold not. intros.
       binds_cases H.
       * subst. unfold dom in Fr0. fsetdec.
-      * subst. 
+      * subst.
         assert (ok (F ++ [(Z, bind_sub P)] ++ E)) by auto.
         exfalso.
         pose proof (fresh_mid_head _ _ _ _ _ H).
@@ -618,8 +694,8 @@ Proof with eauto using wf_cset_narrowing_typ, wf_env_narrowing_typ, cv_narrowing
           (* then use sub_implies_subcapt *)
           destruct (cv_exists E P) as [C CV]...
           { destruct C...
-            ** 
-            
+            **
+
             (* universal *)
                 exfalso. admit.
             ** admit.
